examples/auction/test/test_lib.rs
@@ -1,6 +1,260 @@
-fn test_init_smash_zero () -> bool {
-    match piggy_smash((42, 42, 0, piggy_init())) {
-	Result::Ok ((ctx, owner, balance)) => balance == 0,
-	Result::Err (()) => false,
-    }
+#[cfg(test)]
+extern crate quickcheck;
+#[cfg(test)]
+#[macro_use(quickcheck)]
+extern crate quickcheck_macros;
+
+#[cfg(test)]
+use quickcheck::*;
+
+#[cfg(proof)]
+#[cfg(test)]
+#[quickcheck]
+// #[requires("item === PublicByteSeq::new(0_usize)")]
+#[ensures("result === true")]
+/// Test that the smart-contract initialization sets the state correctly
+/// (no bids, active state, indicated auction-end time and item name).
+pub fn auction_test_init(item: PublicByteSeq, time: u64) -> bool {
+    fresh_state(item.clone(), time)
+        == State(
+            AuctionState::NotSoldYet,
+            0_u64,
+            item.clone(),
+            time,
+            SeqMap(PublicByteSeq::new(0_usize), PublicByteSeq::new(0_usize)),
+        )
+}
+
+#[cfg(test)]
+#[cfg(proof)]
+fn verify_bid(
+    item: PublicByteSeq,
+    state: State,
+    account: UserAddress,
+    ctx: Context,
+    amount: u64,
+    bid_map: SeqMap,
+    highest_bid: u64,
+) -> (State, SeqMap, bool) {
+    let time = 100_u64;
+
+    let t = auction_bid(ctx, amount, state.clone());
+    
+    let (state, res) = match t {
+        AuctionBidResult::Err(e) => (state, false),
+        AuctionBidResult::Ok(s) => (s, true)
+    };
+    
+    let bid_map = match seq_map_update_entry(bid_map.clone(), account, highest_bid) {
+        MapUpdate::Update(_, updated_map) => updated_map,
+    };
+
+    println!("res {}", res);
+    
+    (
+        state.clone(),
+        bid_map.clone(),
+        state.clone()
+            == State(
+                AuctionState::NotSoldYet,
+                highest_bid,
+                item.clone(),
+                time,
+                bid_map.clone(),
+            ),
+    )
+}
+
+// const AUCTION_END: u64 = 1;
+
+// fn new_account() -> AccountAddress {
+//     let account = AccountAddress([0; 32]);
+//     ADDRESS_COUNTER.fetch_add(1, Ordering::SeqCst);
+//     account
+// }
+
+// #[cfg(proof)]
+// fn new_account_ctx() -> (UserAddress, Context) {
+//     let account = new_account();
+//     let ctx = new_ctx(account, account, 1_u64);
+//     (account, ctx)
+// }
+
+// #[cfg(proof)]
+// fn new_ctx(
+//     owner: UserAddress,
+//     sender: UserAddress,
+//     slot_time: u64,
+// ) -> Context {
+//     // let mut ctx = Context;
+//     // ctx.set_sender(Address::Account(sender));
+//     // ctx.set_owner(owner);
+//     // ctx.set_metadata_slot_time(Timestamp::from_timestamp_millis(slot_time));
+//     // ctx
+//     (slot_time, sender)
+// }
+
+#[cfg(proof)]
+#[cfg(test)]
+// #[test]
+/// Test a sequence of bids and finalizations:
+/// 0. Auction is initialized.
+/// 1. Alice successfully bids 0.1 GTU.
+/// 2. Alice successfully bids another 0.1 GTU, highest bid becomes 0.2 GTU
+/// (the sum of her two bids). 3. Bob successfully bids 0.3 GTU, highest
+/// bid becomes 0.3 GTU. 4. Someone tries to finalize the auction before
+/// its end time. Attempt fails. 5. Dave successfully finalizes the
+/// auction after its end time.    Alice gets her money back, while
+/// Carol (the owner of the contract) collects the highest bid amount.
+/// 6. Attempts to subsequently bid or finalize fail.
+#[ensures("result === true")]
+fn test_auction_bid_and_finalize(item: PublicByteSeq) -> bool {
+    let time = 100_u64;
+
+    let amount = 100_u64;
+    let winning_amount = 300_u64;
+    // let big_amount = 500_u64;
+
+    let bid_map = SeqMap(PublicByteSeq::new(0_usize), PublicByteSeq::new(0_usize));
+
+    // initializing auction
+    let state = fresh_state(item.clone(), time); // mut
+
+    // 1st bid: account1 bids amount1
+    let alice = (UserAddress([ 0_u8, 0_u8, 0_u8, 0_u8, 0_u8, 0_u8, 0_u8, 0_u8, 0_u8, 0_u8, 0_u8, 0_u8, 0_u8, 0_u8, 0_u8, 0_u8, 0_u8, 0_u8, 0_u8, 0_u8, 0_u8, 0_u8, 0_u8, 0_u8, 0_u8, 0_u8, 0_u8, 0_u8, 0_u8, 0_u8, 0_u8, 0_u8,]));
+    let alice_ctx = (1_u64, UserAddressSet::UserAddressSome(alice));
+
+    println!("{}", bid_map);
+    
+    let (state, bid_map, result_0) = verify_bid(
+        item.clone(),
+        state,
+        alice,
+        alice_ctx,
+        amount,
+        bid_map,
+        amount,
+    );
+
+    // // 2nd bid: account1 bids `amount` again
+    // // should work even though it's the same amount because account1 simply
+    // // increases their bid
+    let (state, bid_map, result_1) = verify_bid(
+        item.clone(),
+        state,
+        alice,
+        alice_ctx,
+        amount,
+        bid_map,
+        amount + amount,
+    );
+
+    // // 3rd bid: second account
+    let bob = (UserAddress([ 1_u8, 1_u8, 1_u8, 1_u8, 1_u8, 1_u8, 1_u8, 1_u8, 1_u8, 1_u8, 1_u8, 1_u8, 1_u8, 1_u8, 1_u8, 1_u8, 1_u8, 1_u8, 1_u8, 1_u8, 1_u8, 1_u8, 1_u8, 1_u8, 1_u8, 1_u8, 1_u8, 1_u8, 1_u8, 1_u8, 1_u8, 1_u8, ]));
+    let bob_ctx = (2_u64, UserAddressSet::UserAddressSome(bob));
+
+    let (state, bid_map, result_2) = verify_bid(
+        item.clone(),
+        state,
+        bob,
+        bob_ctx,
+        winning_amount,
+        bid_map,
+        winning_amount,
+    );
+
+    // let owner = (UserAddress([
+    //     0_u8, 0_u8, 0_u8, 0_u8, 0_u8, 0_u8, 0_u8, 0_u8, 0_u8, 0_u8, 0_u8, 0_u8, 0_u8, 0_u8, 0_u8,
+    //     0_u8, 0_u8, 0_u8, 0_u8, 0_u8, 0_u8, 0_u8, 0_u8, 0_u8, 0_u8, 0_u8, 0_u8, 0_u8, 0_u8, 0_u8,
+    //     0_u8, 0_u8,
+    // ]));
+
+    // let sender = owner;
+    // let balance = 100_u64;
+    // let ctx4 = (1_u64, owner, balance);
+
+    // let (state, finres) = auction_finalize(ctx4, state);
+
+    // let result_3 = match finres {
+    //     AuctionFinalizeResult::Err(err) => match err {
+    //         FinalizeError::AuctionStillActive => true,
+    //         FinalizeError::BidMapError => false,
+    //         FinalizeError::AuctionFinalized => false,
+    //     },
+    //     AuctionFinalizeResult::Ok(_) => false,
+    // };
+
+    // // // finalizing auction
+    // // let carol = new_account();
+    // let carol = (UserAddress([
+    //     2_u8, 2_u8, 2_u8, 2_u8, 2_u8, 2_u8, 2_u8, 2_u8, 2_u8, 2_u8, 2_u8, 2_u8, 2_u8, 2_u8, 2_u8,
+    //     2_u8, 2_u8, 2_u8, 2_u8, 2_u8, 2_u8, 2_u8, 2_u8, 2_u8, 2_u8, 2_u8, 2_u8, 2_u8, 2_u8, 2_u8,
+    //     2_u8, 2_u8,
+    // ]));
+    // let carol_ctx = (2_u64, UserAddressSet::UserAddressSome(carol));
+
+    // // // let dave = new_account();
+    // // let dave = (UserAddress([
+    // //     3_u8, 3_u8, 3_u8, 3_u8, 3_u8, 3_u8, 3_u8, 3_u8, 3_u8, 3_u8, 3_u8, 3_u8, 3_u8, 3_u8, 3_u8,
+    // //     3_u8, 3_u8, 3_u8, 3_u8, 3_u8, 3_u8, 3_u8, 3_u8, 3_u8, 3_u8, 3_u8, 3_u8, 3_u8, 3_u8, 3_u8,
+    // //     3_u8, 3_u8,
+    // // ]));
+    // // let dave_ctx = (3_u64, UserAddressSet::UserAddressSome(dave));
+
+    // let ctx5 = (2_u64, carol, winning_amount);
+
+    // let (state, finres2) = auction_finalize(ctx5, state);
+
+    // // let result_4 = match finres2 {
+    // //     AuctionFinalizeResult::Err(err) => false,
+    // //     AuctionFinalizeResult::Ok(actions) => true,
+    // // };
+
+    // // let result_4 = state == State (
+    // //     AuctionState::Sold(bob),
+    // //     winning_amount,
+    // //     item.clone(),
+    // //     1_u64,
+    // //     bid_map.clone(),
+    // // );
+
+    // // assert_eq!(state, make_state (
+    // //     AuctionState::Sold(bob),
+    // //     winning_amount,
+    // //     ITEM.as_bytes().to_vec(),
+    // //     Timestamp::from_timestamp_millis(AUCTION_END),
+    // //     bid_map,
+    // // ));
+
+    // // let actions = finres2.expect("Finalizing auction should work");
+    // // assert_eq!(
+    // //     actions,
+    // //     ActionsTree::simple_transfer(&carol, winning_amount)
+    // //         .and_then(ActionsTree::simple_transfer(&alice, amount + amount))
+    // // );
+    // // assert_eq!(state, make_state (
+    // //     AuctionState::Sold(bob),
+    // //     winning_amount,
+    // //     ITEM.as_bytes().to_vec(),
+    // //     Timestamp::from_timestamp_millis(AUCTION_END),
+    // //     bid_map,
+    // // ));
+
+    // // // attempting to finalize auction again should fail
+    // // let finres3: Result<ActionsTree, _> = auction_finalize(&ctx5, &mut state);
+    // // expect_error(
+    // //     finres3,
+    // //     FinalizeError::AuctionFinalized,
+    // //     "Finalizing auction a second time should fail",
+    // // );
+
+    // // // attempting to bid again should fail
+    // // let res4: Result<ActionsTree, _> = auction_bid(&bob_ctx, big_amount, &mut state);
+    // // expect_error(
+    // //     res4,
+    // //     BidError::AuctionFinalized,
+    // //     "Bidding should fail because the auction is finalized",
+    // // );
+
+    result_0 && result_1 && result_2 // && result_3 // && result_4
 }
