coq/src/coverage.v
@@ -27,7 +27,7 @@ Definition eqb_leibniz_enum_typ (x y : enum_typ) : eqb_enum_typ x y = true <-> x
 Proof. split. intros; destruct x ; destruct y ; try (f_equal ; apply eqb_leibniz) ; easy. intros ; subst ; destruct y ; try reflexivity ; try (apply eqb_refl). Qed.
 
 Instance eq_dec_enum_typ : EqDec (enum_typ) :=
-Build_EqDec (enum_typ) (eqb_enum_typ) (eqb_leibniz_enum_typ).
+Build_EqDec (enum_typ) (eqb_enum_typ) (eqb_leibniz_enum_typ) (eqb_leibniz'_enum_typ).
 
 
 Inductive map :=
@@ -42,14 +42,14 @@ Definition eqb_leibniz_map (x y : map) : eqb_map x y = true <-> x = y.
 Proof. split. intros; destruct x ; destruct y ; try (f_equal ; apply eqb_leibniz) ; easy. intros ; subst ; destruct y ; try reflexivity ; try (apply eqb_refl). Qed.
 
 Instance eq_dec_map : EqDec (map) :=
-Build_EqDec (map) (eqb_map) (eqb_leibniz_map).
+Build_EqDec (map) (eqb_map) (eqb_leibniz_map) (eqb_leibniz'_map).
 
 
 Inductive tuple_struct_typ :=
 | TupleStructTyp : (int64 × enum_typ × map) -> tuple_struct_typ.
 
 Definition eqb_tuple_struct_typ (x y : tuple_struct_typ) : bool :=
-  match x with
+match x with
    | TupleStructTyp a => match y with | TupleStructTyp b => a =.? b end
    end.
 
@@ -57,16 +57,14 @@ Definition eqb_leibniz_tuple_struct_typ (x y : tuple_struct_typ) : eqb_tuple_str
 Proof. split. intros; destruct x ; destruct y ; try (f_equal ; apply eqb_leibniz) ; easy. intros ; subst ; destruct y ; try reflexivity ; try (apply eqb_refl). Qed.
 
 Instance eq_dec_tuple_struct_typ : EqDec (tuple_struct_typ) :=
-Build_EqDec (tuple_struct_typ) (eqb_tuple_struct_typ) (eqb_leibniz_tuple_struct_typ).
+Build_EqDec (tuple_struct_typ) (eqb_tuple_struct_typ) (eqb_leibniz_tuple_struct_typ) (eqb_leibniz'_tuple_struct_typ).
 
 
 Definition instance  : tuple_struct_typ :=
-  TupleStructTyp (
-    (
+  TupleStructTyp ((
       @repr WORDSIZE64 0,
       ZeroArg (tt),
-      Map (
-        (
+      Map ((
           seq_new_ (@repr WORDSIZE8 0) (usize 0),
           seq_new_ (@repr WORDSIZE8 0) (usize 0)
         ))
@@ -84,18 +82,14 @@ Definition eqb_leibniz_map_entry (x y : map_entry) : eqb_map_entry x y = true <-
 Proof. split. intros; destruct x ; destruct y ; try (f_equal ; apply eqb_leibniz) ; easy. intros ; subst ; destruct y ; try reflexivity ; try (apply eqb_refl). Qed.
 
 Instance eq_dec_map_entry : EqDec (map_entry) :=
-Build_EqDec (map_entry) (eqb_map_entry) (eqb_leibniz_map_entry).
+Build_EqDec (map_entry) (eqb_map_entry) (eqb_leibniz_map_entry) (eqb_leibniz'_map_entry).
 
 
 Definition map_get_entry (m_0 : map) (entry_1 : arr_typ) : map_entry :=
-  let 'Map ((m0_2, m1_3)) :=
-    m_0 in 
-  let res_4 : map_entry :=
-    Entry (
-      (
+  let 'Map ((m0_2, m1_3)) := m_0 in 
+  let res_4 : map_entry := Entry ((
         @repr WORDSIZE64 0,
-        Map (
-          (
+        Map ((
             seq_concat ((m0_2)) (entry_1),
             seq_concat ((m1_3)) (u64_to_be_bytes (@repr WORDSIZE64 0))
           ))
@@ -103,21 +97,12 @@ Definition map_get_entry (m_0 : map) (entry_1 : arr_typ) : map_entry :=
   let res_4 :=
     foldi (usize 0) ((seq_len ((m0_2))) / (usize 32)) (fun x_5 res_4 =>
       let '(res_4) :=
-        if (
-          array_from_seq (32) (
-            seq_slice ((m0_2)) ((x_5) * (usize 32)) (usize 32))) array_eq (
-          entry_1):bool then (
-          let res_4 :=
-            Entry (
-              (
-                u64_from_be_bytes (
-                  array_from_seq (8) (
-                    seq_slice (m1_3) ((x_5) * (usize 8)) (usize 8))),
+        if (array_from_seq (32) (seq_slice ((m0_2)) ((x_5) * (usize 32)) (usize 32))) array_eq (entry_1):bool then (
+          let res_4 := Entry ((
+                u64_from_be_bytes (array_from_seq (8) (seq_slice (m1_3) ((x_5) * (usize 8)) (usize 8))),
                 Map (((m0_2), (m1_3)))
               )) in 
-          (res_4)
-        ) else ( (res_4)
-        ) in 
+          (res_4) ) else ( (res_4) ) in 
       (res_4))
     res_4 in 
   res_4.
@@ -130,14 +115,10 @@ Definition map_update_entry
   (entry_7 : arr_typ)
   (amount_8 : int64)
   : map_update :=
-  let 'Map ((m0_9, m1_10)) :=
-    m_6 in 
-  let res_11 : map_update :=
-    Update (
-      (
+  let 'Map ((m0_9, m1_10)) := m_6 in 
+  let res_11 : map_update := Update ((
         amount_8,
-        Map (
-          (
+        Map ((
             seq_concat (m0_9) (entry_7),
             seq_concat (m1_10) (u64_to_be_bytes (amount_8))
           ))
@@ -145,24 +126,15 @@ Definition map_update_entry
   let res_11 :=
     foldi (usize 0) ((seq_len ((m0_9))) / (usize 32)) (fun x_12 res_11 =>
       let '(res_11) :=
-        if (
-          array_from_seq (32) (
-            seq_slice ((m0_9)) ((x_12) * (usize 32)) (usize 32))) array_eq (
-          entry_7):bool then (
-          let res_11 :=
-            Update (
-              (
+        if (array_from_seq (32) (seq_slice ((m0_9)) ((x_12) * (usize 32)) (usize 32))) array_eq (entry_7):bool then (
+          let res_11 := Update ((
                 amount_8,
-                Map (
-                  (
+                Map ((
                     seq_update ((m0_9)) ((x_12) * (usize 32)) (entry_7),
-                    seq_update ((m1_10)) ((x_12) * (usize 8)) (
-                      u64_to_be_bytes (amount_8))
+                    seq_update ((m1_10)) ((x_12) * (usize 8)) (u64_to_be_bytes (amount_8))
                   ))
               )) in 
-          (res_11)
-        ) else ( (res_11)
-        ) in 
+          (res_11) ) else ( (res_11) ) in 
       (res_11))
     res_11 in 
   res_11.
@@ -172,62 +144,89 @@ Definition check_if_max
   (increase_14 : int64)
   (entry_15 : arr_typ)
   : tuple_struct_typ :=
-  let 'TupleStructTyp ((max_16, enum_typ_17, map_18)) :=
-    instance_13 in 
-  let '(curr_val_19, map_20) :=
-    match map_get_entry (map_18) (entry_15) with
-    | Entry (curr_val_21, map_22) => (curr_val_21, map_22) end in 
+  let 'TupleStructTyp ((max_16, enum_typ_17, map_18)) := instance_13 in 
+  let '(curr_val_19, map_20) := match map_get_entry (map_18) (entry_15) with
+    | Entry (curr_val_21, map_22) => (curr_val_21, map_22)
+    end in 
   let '(res_val_23, map_24) :=
-    match map_update_entry (map_20) (entry_15) (
-      (increase_14) .+ (curr_val_19)) with
-    | Update (res_val_25, map_26) => (res_val_25, map_26) end in 
-  let enum_typ_27 : enum_typ :=
-    match (enum_typ_17) with
+    match map_update_entry (map_20) (entry_15) ((increase_14) .+ (curr_val_19)) with
+    | Update (res_val_25, map_26) => (res_val_25, map_26)
+    end in 
+  let enum_typ_27 : enum_typ := match (enum_typ_17) with
     | Empty => ZeroArg (tt)
     | ZeroArg tt => OneArg (entry_15)
     | OneArg add_28 => TwoArg ((add_28, @repr WORDSIZE8 0))
-    | TwoArg (add_29, i_30) => TwoArg (
-      (add_29, (i_30) .+ (@repr WORDSIZE8 1))) end in 
-  let 'tt :=
-    if ((enum_typ_27)) =.? (
-      TwoArg ((entry_15, @repr WORDSIZE8 100))):bool then ( tt
-    ) else ( tt
-    ) in 
-  let 'tt :=
-    if (
-      TupleStructTyp (
-        ((increase_14) .+ (res_val_23), (enum_typ_27), (map_24)))) =.? (
-      TupleStructTyp ((max_16, (enum_typ_27), (map_24)))):bool then ( tt
-    ) else ( tt
-    ) in 
-  (
-    if ((max_16) <.? ((increase_14) .+ (res_val_23))):bool then (
-      TupleStructTyp (
-        ((increase_14) .+ (res_val_23), enum_typ_27, map_24))) else (
-      TupleStructTyp ((max_16, enum_typ_27, map_24)))).
+    | TwoArg (add_29, i_30) => TwoArg ((add_29, (i_30) .+ (@repr WORDSIZE8 1)))
+    end in 
+  let 'tt := if ((enum_typ_27)) =.? (TwoArg ((entry_15, @repr WORDSIZE8 100
+        ))):bool then ( tt ) else ( tt ) in 
+  let 'tt := if (TupleStructTyp ((
+          (increase_14) .+ (res_val_23),
+          (enum_typ_27),
+          (map_24)
+        ))) =.? (TupleStructTyp ((max_16, (enum_typ_27), (map_24)))):bool then (
+      tt ) else ( tt ) in 
+  (if ((max_16) <.? ((increase_14) .+ (res_val_23))):bool then (TupleStructTyp ((
+          (increase_14) .+ (res_val_23),
+          enum_typ_27,
+          map_24
+        ))) else (TupleStructTyp ((max_16, enum_typ_27, map_24)))).
 
 Notation "'res_type'" := ((result int64 unit)) : hacspec_scope.
 
 Definition loop_with_early_return (amount_31 : uint_size) : res_type :=
-  let res_32 : (result int64 unit) :=
-    Ok (@repr WORDSIZE64 0) in 
-  match (
-    foldibnd (usize 0) to (usize 100) for res_32>> (fun x_33 res_32 => ifbnd (
-      (x_33) + (amount_31)) >.? (usize 200) : bool
-    thenbnd (
-      match Err (tt)  : result int64 _ with
+  let res_32 : (result int64 unit) := Ok (@repr WORDSIZE64 0) in 
+  match (foldibnd (usize 0) to (usize 100) for res_32>> (fun x_33 res_32 =>
+    ifbnd ((x_33) + (amount_31)) >.? (usize 200) : bool
+    thenbnd (match Err (tt)  : result int64 _ with
        | Err a => Err a
        | Ok _ => Ok (tt)
       end)
     else (tt) >> (fun 'tt =>
-    let '(res_32) :=
-      if (x_33) <.? (usize 50):bool then (
-        let res_32 :=
+    let '(res_32) := if (x_33) <.? (usize 50):bool then ( let res_32 :=
           Ok (pub_u64 (x_33)) in 
-        (res_32)
-      ) else ( (res_32)
-      ) in 
+        (res_32) ) else ( (res_32) ) in 
     Ok ((res_32))))) with
   | Err e => Err e
   | Ok res_32 =>  res_32 end.
+
+Notation "'strange_result'" := ((result int64 unit)) : hacspec_scope.
+
+Definition strange  : strange_result :=
+  match Err (tt)  : result int64 _ with
+   | Err a => Err a
+   | Ok _ => Ok (@repr WORDSIZE64 2)
+  end.
+
+Notation "'loop_result'" := ((result int64 unit)) : hacspec_scope.
+
+Definition loopres  : loop_result :=
+  let result_34 : int64 := @repr WORDSIZE64 1 in 
+  match (foldibnd (usize 1) to (usize 24) for result_34>> (fun x_35 result_34 =>
+    let result_34 := (result_34) .+ (pub_u64 (x_35)) in 
+    ifbnd (result_34) >.? (@repr WORDSIZE64 100) : bool
+    thenbnd (match Err (tt)  : result int64 _ with
+       | Err a => Err a
+       | Ok _ => Ok (tt)
+      end)
+    else (tt) >> (fun 'tt =>
+    Ok ((result_34))))) with
+  | Err e => Err e
+  | Ok result_34 =>  Ok (result_34) end.
+
+Notation "'difficult_result'" := ((result int64 unit)) : hacspec_scope.
+
+Definition difficult  : difficult_result :=
+  let result_36 : uint_size := usize 1 in 
+  match (foldibnd (usize 1) to (usize 24) for result_36>> (fun x_37 result_36 =>
+    let result_36 := (result_36) + (x_37) in 
+    ifbnd (result_36) >.? (usize 100) : bool
+    thenbnd (match Err (tt)  : result int64 _ with
+       | Err a => Err a
+       | Ok _ => Ok (tt)
+      end)
+    else (tt) >> (fun 'tt =>
+    Ok ((result_36))))) with
+  | Err e => Err e
+  | Ok result_36 =>  Ok (result_36) end.
 
